Common/CBase.v
@@ -953,6 +953,33 @@ Lemma ctrans_inj `{CTransSimpl T F} {n m : T} (e e' : n = m) (a b : F n):
 Proof. rewrite <- ctrans_sym. simp ctrans. reflexivity. Qed.
 #[export] Hint Rewrite @ctrans_inj using tc_solve : ctrans.
 
+
+(** ** Computable transport combinators *)
+
+Instance pair_ctrans `{CTrans A F, CTrans A G} :
+    CTrans (λ x, F x * G x)%type | 100 :=
+  λ a b e '(x, y), (ctrans e x, ctrans e y).
+
+Instance pair_ctrans_simpl `{CTransSimpl A F, CTransSimpl A G} :
+  CTransSimpl (λ x, F x * G x)%type | 100.
+Proof. intros x p []. cbn. by simp ctrans. Qed.
+
+Instance pair_ctransl `{EqDecision A, CTrans A F} T :
+    CTrans (λ x, F x * T)%type | 50 :=
+  λ a b e '(x, y), (ctrans e x, y).
+
+Instance pair_ctransl_simpl `{EqDecision A, CTransSimpl A F} T :
+  CTransSimpl (λ x, F x * T)%type | 50.
+Proof. intros x p []. cbn. by simp ctrans. Qed.
+
+Instance pair_ctransr `{EqDecision A, CTrans A F} T :
+    CTrans (λ x, T * F x)%type | 50 :=
+  λ a b e '(x, y), (x, ctrans e y).
+
+Instance pair_ctransr_simpl `{EqDecision A, CTransSimpl A F} T :
+  CTransSimpl (λ x, T * F x)%type | 50.
+Proof. intros x p []. cbn. by simp ctrans. Qed.
+
 (** ** Computable transport for [fin] *)
 
 Arguments eq_add_S {_ _} _.
